Foundation/FirstOrder/Arithmetic/ISigma1/Prenex.lean
@@ -19,18 +19,18 @@ namespace LO.FirstOrder.Arithmetic.ISigma1
 variable {n : ℕ} {φ : ArithmeticSemisentence n} {σ : ArithmeticSentence}
 
 lemma hasPrenex (h : Hierarchy 𝚺 1 φ) :
-    ∃ π : Prenex 𝚺 1 Empty n, 𝗜𝚺₁ ⊢ ∀¹* (φ 🡘 π.val) :=
+    ∃ φ' : Prenex 𝚺 1 Empty n, 𝗜𝚺₁ ⊢ ∀¹* (φ 🡘 φ'.val) :=
   exists_prenex_of_hierarchy 𝗜𝚺₁ h
 
 lemma exists_matrix_provable (h : Hierarchy 𝚺 1 φ) :
     ∃ θ : ArithmeticSemisentence (n + 1), Hierarchy 𝚺 0 θ ∧ 𝗜𝚺₁ ⊢ ∀¹* (φ 🡘 ∃¹ θ) := by
-  obtain ⟨π, hπ⟩ := hasPrenex h;
-  exact ⟨π.sigmaInv.val, π.sigmaInv.val_deltaZero, Prenex.provable_iff_sigmaInv hπ⟩
+  obtain ⟨φ', hφ'⟩ := hasPrenex h;
+  exact ⟨φ'.sigmaInv.val, φ'.sigmaInv.val_deltaZero, Prenex.provable_iff_sigmaInv hφ'⟩
 
 lemma exists_matrix_provable_pi (h : Hierarchy 𝚷 1 φ) :
     ∃ θ : ArithmeticSemisentence (n + 1), Hierarchy 𝚺 0 θ ∧ 𝗜𝚺₁ ⊢ ∀¹* (φ 🡘 ∀¹ θ) := by
-  obtain ⟨π, hπ⟩ := exists_prenex_of_hierarchy 𝗜𝚺₁ h
-  exact ⟨π.piInv.val, π.piInv.val_hierarchy, Prenex.provable_iff_piInv hπ⟩
+  obtain ⟨φ', hφ'⟩ := exists_prenex_of_hierarchy 𝗜𝚺₁ h
+  exact ⟨φ'.piInv.val, φ'.piInv.val_hierarchy, Prenex.provable_iff_piInv hφ'⟩
 
 lemma exists_matrix_provable_of_sentence (h : Hierarchy 𝚺 1 σ) :
     ∃ θ : ArithmeticSemisentence 1, Hierarchy 𝚺 0 θ ∧ 𝗜𝚺₁ ⊢ σ 🡘 ∃¹ θ :=
