Foundation/FirstOrder/Arithmetic/PA/Prenex.lean
@@ -19,26 +19,26 @@ namespace LO.FirstOrder.Arithmetic.Peano
 variable {Γ : Polarity} {s n : ℕ} {φ : ArithmeticSemisentence n} {σ : ArithmeticSentence}
 
 lemma hasPrenex (h : Hierarchy Γ s φ) :
-    ∃ π : Prenex Γ s Empty n, 𝗣𝗔 ⊢ ∀¹* (φ 🡘 π.val) :=
+    ∃ φ' : Prenex Γ s Empty n, 𝗣𝗔 ⊢ ∀¹* (φ 🡘 φ'.val) :=
   exists_prenex_of_hierarchy 𝗣𝗔 h
 
 lemma exists_matrix_provable (h : Hierarchy Γ s φ) :
     ∃ φ₀ : 𝚺₀.Semisentence (n + s), 𝗣𝗔 ⊢ ∀¹* (φ 🡘 φ₀.val.toPrenex Γ s) := by
-  obtain ⟨π, hπ⟩ := hasPrenex h;
-  exact ⟨π.matrix, hπ⟩
+  obtain ⟨φ', hφ'⟩ := hasPrenex h;
+  exact ⟨φ'.matrix, hφ'⟩
 
 lemma exists_matrix_provable_of_sentence (h : Hierarchy Γ s σ) :
-    ∃ π₀ : 𝚺₀.Semisentence (0 + s), 𝗣𝗔 ⊢ σ 🡘 π₀.val.toPrenex Γ s :=
+    ∃ φ₀ : 𝚺₀.Semisentence (0 + s), 𝗣𝗔 ⊢ σ 🡘 φ₀.val.toPrenex Γ s :=
   exists_matrix_provable h
 
 lemma exists_hierarchy_provable_of_sentence (h : Hierarchy 𝚺 (s + 1) σ) :
     ∃ θ : ArithmeticSemisentence 1, Hierarchy 𝚷 s θ ∧ 𝗣𝗔 ⊢ σ 🡘 ∃¹ θ := by
-  obtain ⟨π, hπ⟩ := hasPrenex h;
-  exact ⟨π.sigmaInv.val, π.sigmaInv.val_hierarchy, Prenex.provable_iff_sigmaInv hπ⟩
+  obtain ⟨φ', hφ'⟩ := hasPrenex h;
+  exact ⟨φ'.sigmaInv.val, φ'.sigmaInv.val_hierarchy, Prenex.provable_iff_sigmaInv hφ'⟩
 
 lemma exists_hierarchy_provable_of_sentence_pi (h : Hierarchy 𝚷 (s + 1) σ) :
     ∃ θ : ArithmeticSemisentence 1, Hierarchy 𝚺 s θ ∧ 𝗣𝗔 ⊢ σ 🡘 ∀¹ θ := by
-  obtain ⟨π, hπ⟩ := hasPrenex h;
-  exact ⟨π.piInv.val, π.piInv.val_hierarchy, Prenex.provable_iff_piInv hπ⟩
+  obtain ⟨φ', hφ'⟩ := hasPrenex h;
+  exact ⟨φ'.piInv.val, φ'.piInv.val_hierarchy, Prenex.provable_iff_piInv hφ'⟩
 
 end LO.FirstOrder.Arithmetic.Peano
